GAAARG universe inconsistency.

model.v
@@ -1,7 +1,11 @@
-Require Import ZArith NArith List ListSet Paco.paco.
+Require Import ZArith NArith List ListSet.
 Import ListNotations.
 Definition Name := nat.
 Notation "'dec_type' T" := (forall x y : T, {x=y}+{x<>y}) (at level 70, no associativity).
+
+Ltac split_refl eq_dec a := let H:= fresh in destruct (eq_dec a a) as [H|bad]; [clear H|contradict bad]; auto.
+Ltac split_refl2 eq_dec a a' := let H:= fresh in
+                                destruct (eq_dec a a') as [bad|H]; [contradict bad|clear H]; auto.
 
 Definition name_eq_dec : dec_type Name.
   decide equality.
@@ -28,36 +32,12 @@ Definition Env := list (Name * Addr).
 Definition env_eq_dec : dec_type Env.
   apply list_eq_dec; decide equality; try solve [apply name_eq_dec | apply addr_eq_dec].
 Defined.
-(*
-Inductive sexp :=
-  | atom : Addr -> sexp
-  | lst : sexps -> sexp
-with sexps :=
-       | snil : sexps
-       | scons : sexp -> sexps -> sexps.
-Scheme sexp_ind_2 := Induction for sexp Sort Prop
-                     with sexps_ind_2 := Induction for sexps Sort Prop.
-Combined Scheme sexp_mutind from sexp_ind_2, sexps_ind_2.
-Lemma sexp_eq_dec : forall (s s': sexp) (ss ss' : sexps), (s = s' \/ s <> s') /\ (ss = ss' \/ ss <> ss').
-Proof.
-  Check sexp_mutind.
-  intro s; apply (sexp_mutind (fun s' => s = s' \/ s <> s'));
-  induction s;
-  try solve
-    [intro a0; destruct (addr_eq_dec a a0); [left|right;injection]; congruence
-    | right; discriminate].
-  intros s0 Hdec;
-    pose (Hdec0 := (Hdec (lst s0) s s0));
-    inversion Hdec0 as ([Heq|Hneq] & [Heqs|Hneqs]); firstorder.
-  induction s'.
-  destruct (addr_eq_dec a a0).
-*)
 
 Inductive val :=
   | closure : Name -> Expr -> Env -> val
   | adelay : Addr -> val
-  | amany : set val -> val.
-Definition AbsVal := set val.
+  | amany : list val -> val.
+Definition AbsVal := list val.
 Axiom val_eq_dec : dec_type val.
 Definition absval_eq_dec : dec_type AbsVal.
   apply list_eq_dec,val_eq_dec.
@@ -102,24 +82,40 @@ Definition cesk_eq_dec : dec_type CESK.
   decide equality; try solve [apply kont_eq_dec | apply time_eq_dec | apply ces_point_eq_dec].
 Defined.
 
-Inductive InDom {A B} : list (A * B) -> A -> Prop :=
+Inductive InDom {A B} : list (A * B) -> A -> Type :=
   | dom_fst : `{InDom ((a,b)::rst) a}
   | dom_rst : `{InDom l a -> InDom ((a',b')::l) a}.
 
-Inductive MapsTo {A B} : list (A * B) -> A -> B -> Prop :=
+Inductive MapsTo {A B} : list (A * B) -> A -> B -> Type :=
   | map_fst : `{MapsTo ((a,b)::rst) a b}
   | map_rst : `{a <> a' -> MapsTo l a b -> MapsTo ((a',b')::l) a b}.
 
-Inductive Unmapped {A B} : list (A * B) -> A -> Prop :=
+Inductive Unmapped {A B} : list (A * B) -> A -> Type :=
   | unil : forall a, Unmapped nil a
   | ucons : forall a a' b l, Unmapped l a' -> a <> a' -> Unmapped ((a,b)::l) a'.
+
+Inductive Functional {A B} : list (A * B) -> Type :=
+  | empty_fn : Functional nil
+  | extend_fn : `{Functional l -> Unmapped l a -> Functional ((a,b)::l)}.
+
+Inductive InT {A} : A -> list A -> Type :=
+  in_fst : forall a l, InT a (a :: l)
+| in_rst : forall a l b, InT a l -> InT a (b :: l).
+
+Lemma MapsTo_In : forall A B (l : list (A * B)) a b (H: MapsTo l a b), InT (a,b) l.
+Proof.
+  induction l as [|(a,b) l' IH];
+  intros a' b' H; inversion H; (* finishes base case *)
+  subst; [constructor|right; apply IH]; auto.
+Qed.
 
 Theorem unmapped_not_mapped : forall A B
                                      (eq_dec : dec_type A)
                                      (l : list (A*B)) a,
-                              Unmapped l a <-> forall b, ~ MapsTo l a b.
+                                (Unmapped l a -> forall b, MapsTo l a b -> False) *
+                                ((forall b, (MapsTo l a b -> False)) -> Unmapped l a).
 Proof.
-  intros A B eq_dec l a; induction l as [|(a',b') l'];
+  intros A B eq_dec l a; induction l as [|(a',b') l' [IHl'0 IHl'1]];
   split;
   [intros H b bad; inversion bad
   |constructor
@@ -127,20 +123,48 @@ Proof.
     inversion H as [| ? ? ? ? Hunmapped Hbad];
     inversion bad as [| ? ? ? ? ? ? Hbadmap]; subst;
     [contradict Hbad; reflexivity
-    | rewrite IHl' in Hunmapped; apply Hunmapped in Hbadmap; auto]
+    |specialize IHl'0 with Hunmapped; apply IHl'0 in Hbadmap]  
   |intros H; constructor;
-  [rewrite IHl'; intros bb bad; destruct (eq_dec a a'); subst;
+  [apply IHl'1; intros bb bad; destruct (eq_dec a a'); subst;
       [pose (HC := (H b')); contradict HC; constructor
       |pose (HC := (H bb)); contradict HC; constructor; auto]
-     |intro Heq; subst; apply H with (b := b'); constructor]].
+     |intro Heq; subst; apply H with (b := b'); constructor]]; auto.
 Qed.
+
+Lemma in_not_unmapped : forall A B (l : list (A * B)) a b (H:InT (a,b) l), Unmapped l a -> False.
+Proof.
+  induction l as [|(a,b) l' IH]; intros a0 b0 H bad; inversion H; subst;[
+  inversion bad; intuition
+  |inversion bad as [|? ? ? ? bad']; apply IH with (b:= b0) in bad'; auto].
+Qed.
+
+Lemma in_functional_mapsto : forall A B (eq_dec : dec_type A) (l : list (A * B)) (F : Functional l)
+                                    a b (H : InT (a,b) l), MapsTo l a b.
+Proof.
+  induction l as [|(a,b) l' IH];
+  intros F a' b' H; inversion H;[ (* finishes base case *)
+    subst; constructor; auto
+  |inversion F as [|? ? ? Hfun Hunmapped]; subst;
+   destruct (eq_dec a a'); [subst; contradict Hunmapped; apply in_not_unmapped with (b:=b')
+                           |constructor]]; auto.
+Qed.
+
+Remark functional_exchange : forall A B (l : list (A * B)) a b (F: Functional ((a,b)::l)) b', Functional ((a,b')::l).
+Proof. intros; inversion F; constructor; auto. Qed.
 
 Definition in_aval := In.
 
-Definition in_list_list {A B} (l : list (A * (set B))) (a : A) (b : B) : Prop :=
-  exists bs, In (a,bs) l /\ set_In b bs.
+Inductive exT {A} : (A -> Type) -> Type :=
+  exT_intro : forall a P, (P a) -> exT P.
+Notation "'existsT' x .. y , p" := (exT (fun x => .. (exT (fun y => p)) ..))
+  (at level 200, x binder, right associativity,
+   format "'[' 'existsT'  '/  ' x  ..  y ,  '/  ' p ']'").
 
-Inductive in_force (σ : Store) : forall (v v' : val), Prop :=
+
+Definition in_list_list {A B} (l : list (A * (list B))) (a : A) (b : B) : Type :=
+  existsT bs, prod (MapsTo l a bs) (InT b bs).
+
+Inductive in_force (σ : Store) : forall (v v' : val), Type :=
 | forced : `{in_force σ v v}
 | do_force : `{MapsTo σ a vs -> in_aval v' vs -> in_force σ v' (adelay a)}.
 
@@ -162,7 +186,8 @@ Fixpoint lookup_map {A B} (eq_dec : (dec_type A)) (a : A) (ρ : list (A * B)) : 
   end.
 
 Theorem lookup_mapsto : forall A B (eq_dec : dec_type A) (l : list (A * B)) a b,
-                          MapsTo l a b <-> (lookup_map eq_dec a l) = Some b.
+                          prod ((MapsTo l a b) -> (lookup_map eq_dec a l) = Some b)
+                               ((lookup_map eq_dec a l) = Some b -> (MapsTo l a b)).
 Proof.
   induction l as [|(a,b) l' IH]; [intros a b; split; intro Hvac; inversion Hvac|].
   intros a' b'; split; intro H; simpl in *;
@@ -179,79 +204,242 @@ Qed.
 Definition lookup_ρ := lookup_map name_eq_dec (B := Addr).
 Definition lookup_σ := lookup_map addr_eq_dec (B := AbsVal).
 
-Fixpoint list_join {A B C}
-         (eq_dec : dec_type A)
-         (combine : list (A * B) -> B -> C -> B)
-         (base : list (A * B) -> C -> B)
-         (l_orig : list (A * B))
+Section ListJoin.
+Variables (A B C : Type) (eq_dec : dec_type A)
+          (combine : list (A * B) -> B -> C -> B)
+          (base : list (A * B) -> C -> B).
+Fixpoint list_join  (l_orig : list (A * B))
          (a : A) (c : C)
          (l : list (A * B)) : list (A * B) :=
   match l with
       | nil => (a,base l_orig c)::nil
       | (a',b)::l' => if (eq_dec a a') then
                         (a,(combine l_orig b c))::l'
-                      else (a',b)::(list_join eq_dec combine base l_orig a c l')
+                      else (a',b)::(list_join l_orig a c l')
   end.
+Definition singleton {A} (eq_dec : dec_type A) (x : A) : list A := set_add eq_dec x (empty_set _).
+End ListJoin.
 
+Section ListJoin_facts.
+Variables (A C : Type) (eq_dec : dec_type A)
+          (combine : list (A * list C) -> list C -> C -> list C)
+          (base : list (A * list C) -> C -> list C)
+          (Hextensive : (forall l b c, InT c (combine l b c)))
+          (Hsingleton : (forall l c, InT c (base l c))).
 Lemma in_list_join :
-  forall A B (combine : list (A * set B) -> set B -> B -> set B) base l l' a c
-    (eq_dec : dec_type A),
-    (forall l b c, set_In c (combine l b c)) ->
-    (forall l c, set_In c (base l c)) ->
-    (forall ab, In ab l -> In ab l') ->
+  forall l l' a c,
+    (forall ab, InT ab l -> InT ab l') ->
   in_list_list (list_join eq_dec combine base l' a c l) a c.
 Proof.
-  intros A B combine base l l' a c eq_dec Hextensive Hsingleton Hcontain.
+  intros l l' a c Hcontain.
   induction l; simpl.
   exists (base l' c); split; [left| apply Hsingleton]; auto.
   destruct a0 as [a' b]; destruct (eq_dec a a') as [Heq | Hneq];
-  [subst; exists (combine l' b c); split; [left|apply Hextensive]; auto
-  |].
-  destruct IHl as [bs [Hainbs Hbinbs]].
-   (* backchain IHl *)
-    intros (a_,bs') Hin; apply Hcontain; right; auto.
-  exists bs; split; [right|]; auto.
+  [subst; exists (combine l' b c); split; [left|apply Hextensive]
+  |assert (IHneed : (forall ab, InT ab l -> InT ab l')) by (intros (a_,bs') Hin; apply Hcontain; right; auto);
+    set (mumble := (IHl IHneed));
+    inversion mumble as [wit P Hwit Heq]; subst; destruct Hwit as [Hmap Hin];
+    exists wit; split; [apply map_rst|]]; auto.
 Qed.
 
+Lemma unmapped_join : `{Unmapped l a -> a <> a' -> Unmapped (list_join eq_dec combine base l' a' c l) a}.
+Proof.
+  induction l as [|(a,b) l_ IH]; intros a0 a' l' c H ?;
+  simpl; repeat constructor; auto.
+  simpl; destruct (eq_dec a' a) as [Heq|Hneq];
+  [subst; inversion H; constructor
+  |constructor;inversion H;[apply IH|]];auto.
+Qed.
+
+Lemma functional_join : `{Functional l -> Functional (list_join eq_dec combine base l' a c l)}.
+Proof.
+  induction l as [|(a,b) l_ IH]; simpl;
+  [intros; repeat constructor
+  |intros l' a' c F].
+  destruct (eq_dec a' a) as [Heq|Hneq];
+  [subst; apply functional_exchange with (b := b)
+  |constructor; inversion F; [apply IH|apply unmapped_join]]; auto.
+Qed.
+
+Variable Hextensive' : (forall l b c c', InT c' b -> InT c' (combine l b c)).
 Lemma in_list_join2 :
-  forall A B (combine : list (A * set B) -> set B -> B -> set B) base l l' a a' c c'
-    (eq_dec : dec_type A),
-    (forall l b c c', set_In c' b -> set_In c' (combine l b c)) ->
-    (forall l b c, set_In c (combine l b c)) ->
-    (forall l c, set_In c (base l c)) ->
-    (forall ab, In ab l -> In ab l') ->
+  forall l l' a a' c c',
   in_list_list l a' c' ->
   in_list_list (list_join eq_dec combine base l' a c l) a' c'.
 Proof.
-  intros A B combine base l l' a a' c c' eq_dec Hextensive1 Hextensive2 Hsingleton Hcontain Hold.
+  intros l l' a a' c c' Hold;
   induction l; simpl;
-  inversion Hold as [bs [Hpairin Hsetin]];
+  inversion Hold as [bs ? Hwit]; destruct Hwit as [Hpairin Hsetin]; subst;
   [(* base case *) inversion Hpairin
   |destruct a0; destruct (eq_dec a a0) as [Heq | Hneq]; subst;
    [(* Heq *)
-     destruct (eq_dec a0 a') as [Heq' | Hneq']; subst;
-    [(* Heq' *)
-      inversion Hpairin as [Hpeq|Hrest];[
-        injection Hpeq; intros; subst;
-        exists (combine l' bs c); split; [left; auto|apply Hextensive1]
-       |exists bs; split; [right|]]; auto
-    |(* Hneq' *)
-      inversion Hpairin as [Hbad|Hrest]; [
-        injection Hbad; intros; subst; contradict Hneq'|
-        exists bs; split; [right|]]; auto]
-    |(* Hneq *)]].
-  destruct (eq_dec a0 a') as [Heq' | Hneq']; subst;
-  inversion Hpairin as [Hpeq|Hrest]; try solve
-  [ (* Heq', Hpeq *)
-    injection Hpeq; intros; subst;
-      exists bs; split; [left|]; auto
-   |(* Heq', Hrest *)
-   assert (Hneed : in_list_list l a' c') by (exists bs; split; auto);
-     assert (Hcontain' : forall ab, In ab l -> In ab l') by (intros ab Hin; apply Hcontain; right; auto);
-     destruct (IHl Hcontain' Hneed) as [bs' [H0 H1]]; exists bs'; split; [right|]; auto].
+     subst; inversion Hpairin; subst;
+    [exists (combine l' bs c); split; [left|apply Hextensive']; auto
+           |exists bs; split; [right|]; auto]
+   |(* Hneq *)
+    destruct (eq_dec a0 a') as [Heq' | Hneq'];
+     inversion Hpairin as [|? ? ? ? ? ? Hmap']; subst;
+    [exists bs; split; [constructor|]; auto
+    |match goal with [Hbad : ?a <> ?a |- _] => contradict Hbad; auto end
+    |exists bs; constructor; [constructor|]; auto
+    |assert (IHneed : in_list_list l a' c') by (exists bs; repeat constructor; auto);
+     set (IHl_ := IHl IHneed);
+     inversion IHl_ as [x ? Hwit]; destruct Hwit as [Hmap Hin];
+     exists x; repeat constructor; auto]]].
 Qed.
 
-Definition singleton {A} (eq_dec : dec_type A) (x : A) : set A := set_add eq_dec x (@empty_set A).
+Lemma non_join_untouched : forall l l' a a' c b
+                             (Hneq : a <> a')
+                             (H: MapsTo (list_join eq_dec combine base l' a c l) a' b),
+                             MapsTo l a' b.
+Proof.
+  induction l as [|(a_,b_) l_ IH]; intros;
+  [inversion H; subst; [contradict Hneq|]; auto
+  |
+  simpl in H; inversion H as [? ? rst H'|? a'' ? ? ? Hneq'' map' Hinj]; subst;
+  destruct (eq_dec a a_) as [Heq_|Hneq_];
+  try (injection H'; intros; subst);
+  try (injection Hinj; intros; subst);
+  [
+  (* Eq *)
+  constructor; [auto
+               |apply IH with (l' := l') (a := a_) (c := c);
+                 [auto
+                 |contradict Hneq; auto]]
+  |constructor
+  |subst; constructor; auto
+  |constructor; [auto | apply IH with (l' := l') (a := a) (c := c); auto]]].
+Qed.
+
+(*
+  
+Lemma unmapped_join2 : forall l a a' b c l'
+                             (Hcontain : (forall a c, in_list_list l a c -> in_list_list l' a c)
+                                          \/ (b = (base l' c))),
+                        Unmapped l a' ->
+                        MapsTo (list_join eq_dec combine base l' a c l) a' b ->
+                        (b = (base l' c)) /\ a = a'.
+Proof.
+  induction l as [|(a_,b_) l_ IH];
+  simpl; intros a a' b c l' Hcontain Hunmap Hmap;
+  [inversion Hmap as [|? ? ? ? ? ? Hbad]; subst; split; solve [auto|reflexivity|inversion Hbad]
+  |].
+  destruct (eq_dec a a_) as [Heq | Hneq];
+    [inversion Hunmap as [|? ? ? ? Hunmap' Hneq]; subst;
+     inversion Hmap as [|? ? ? ? ? ? Hbad]; split; try solve [reflexivity|
+                                             rewrite unmapped_not_mapped in Hunmap';
+                                             [apply Hunmap' in Hbad; contradiction
+                                             |auto]]
+    |].
+  inversion Hmap as [|? ? ? ? ? ? Hbad]; subst; contradict Hneq; auto.
+  apply IH with (b := b) (c := c) (l' := l').
+  inversion Hcontain as [L|R].
+  specialize L with a_ b_
+  intros a_' c_' Hin; inversion Hin as [bs_ [Hmap_ Hsetin_]];
+  apply Hcontain; destruct (eq_dec a_' a_) as [Heq_|Hneq_];
+  [subst
+    |exists bs_; repeat constructor]; auto.
+  unfold in_list_list.
+  Focus 2.
+  
+    [intros a_' c_' Hin
+    |inversion Hunmap
+    |]; auto.
+
+; 
+  inversion Hmap; [(* a_' = a_ *)
+                   rewrite unmapped_not_mapped in Hunmap; [
+                    (* rewritten *)
+                    subst; match goal with [bad : ?a <> ?a |- _] => contradict bad; auto end
+                    |(* satisfy hyp *)assumption]
+                   |subst]. 
+  Check unmapped_not_mapped.
+                       
+   [specialize Hunmap with b; contradict Hunmap; constructor
+   |assumption
+   |
+   |assumption].
+  .
+  ; constructor; auto | auto].
+    
+
+ subst; repeat constructor|]
+  constructor.
+Qed.
+Admitted.*)
+Theorem set_add_intro1T : forall (a b : A) (l : list A), InT a l -> InT a (set_add eq_dec b l).
+Proof.
+  clear; induction l as [|x l' IH]; intros H; inversion H; subst; simpl;
+  destruct (eq_dec b x); subst; constructor; auto.
+Qed.
+
+Theorem set_add_intro2T : forall (a : A) (l : list A), InT a (set_add eq_dec a l).
+Proof.
+  clear; induction l as [|x l' IH]; subst; simpl;[
+    constructor
+    |destruct (eq_dec a x); subst; constructor; auto].
+Qed.
+
+Theorem set_add_elimT : forall (a b : A) (l : list A) (H: InT a (set_add eq_dec b l)),
+          (a = b) + (InT a l).
+Proof.
+  clear.
+  induction l; intros; simpl in H; inversion H as [? l_|? l' b' Hin]; subst; try solve [intuition];
+  destruct (eq_dec b a0) as [Heq | Hneq];
+  try match goal with [H : ?a :: ?l = ?b :: ?k |- _] => injection H; intros; subst end;
+  try solve
+  [right; constructor | right; auto].
+  set (IHl_ := IHl Hin).
+  inversion IHl_; [left|right;constructor]; auto.
+Qed.
+
+End ListJoin_facts.
+Section ListJoin_morefacts.
+Variables (A C : Type) (eq_dec : dec_type A) (ceq_dec : dec_type C).
+Definition joiner := (fun (_ : list (A * list C)) κs κ => (set_add ceq_dec κ κs)).
+Definition singler := (fun (_ : list (A * list C)) c => (singleton ceq_dec c)).
+Hint Unfold singleton singler.
+
+Lemma in_list_join_set_split : forall (l l' : list (A * list C))
+                                      (a a' : A)
+                                      (c c' : C)
+                                 (Hin : in_list_list (list_join eq_dec joiner singler l' a c l) a' c'),
+                                 sum (prod (a = a') (c = c')) (in_list_list l a' c').
+Proof.
+  induction l as [|(a,cs) l_ IH]; [intros|intros ll' aa aa' cc cc' Hin];
+  simpl in *; 
+  inversion Hin as [cs_ ? Hwit]; destruct Hwit as [map_ in_]; subst;
+  [(* base case *)
+  inversion map_ as [|? ? ? ? ? ? bad]; subst;
+    [inversion in_ as [|? ? ? bad]; subst; [left; split; auto|inversion bad]
+    |inversion bad]
+  |].
+  destruct (eq_dec aa a) as [Heq|Hneq];
+    inversion map_ as [|foo bar baz qux moo boo too];subst.
+
+  (* Eq case with inversion *)
+  destruct (set_add_elimT ceq_dec _ _ in_) as [Hceq|Hinrest];
+       [intuition
+       |subst; right; exists cs; repeat constructor; auto].
+
+  right; exists cs_; repeat constructor; auto.
+
+  (* Neq case with inversion *)
+  right; exists cs_; repeat constructor; auto.
+
+  destruct (eq_dec aa aa') as [Heq_|Hneq_].
+  (* eq *)
+  destruct IH with (l' := ll') (a := aa) (a' := aa') (c := cc) (c' := cc') as [S|S];
+    [exists cs_; constructor; auto
+    |left; exact S
+    |inversion S as [ccs ? Hwit]; destruct Hwit as [mmap min]; right; exists ccs; split;[constructor|];auto].
+  (* neq *)
+  right.
+  apply non_join_untouched with (eq_dec := eq_dec) (combine := joiner) (base := singler) in too;
+    [exists cs_; repeat constructor|]; auto.
+Qed.
+    
+End ListJoin_morefacts.
 
 Definition force (σ : Store) (v:val) : AbsVal :=
   match v with
@@ -270,54 +458,46 @@ Definition σ_join (σ : Store) (a : Addr) (v : val) : Store :=
             (fun σ_orig vs v => (absval_join vs (force σ_orig v)))
             force σ a v σ.
 Section StandardSemantics.
-Variable alloc : CESK -> Addr.
-Variable tick : CESK -> Time.
+Variable alloc : CES_point -> Store -> Addr.
+Variable tick : CES_point -> Store -> Time.
 Variable time0 : Time.
 
-Inductive red_cesk : CESK -> CESK -> Prop :=
-  ev_var : `{let s := (shell (ev (var x) ρ σ) κ t) in
+Inductive red_cesk : CESK -> CESK -> Type :=
+  ev_var : `{let p := (ev (var x) ρ σ) in
              MapsTo ρ x a ->
-             red_cesk s (shell (co (adelay a) σ) κ (tick s))}
-| ev_app : `{let s := (shell (ev (app e0 e1) ρ σ) κ t) in
-             red_cesk s (shell (ev e0 ρ σ) ((ar e1 ρ)::κ) (tick s))}
-| ev_lam : `{let s := (shell (ev (lam x e) ρ σ) κ t) in
-             red_cesk s (shell (co (closure x e ρ) σ) κ (tick s))}
-| co_ar : `{let s := (shell (co v σ) ((ar e ρ)::κ) t) in
-            red_cesk s (shell (ev e ρ σ) ((fn v)::κ) (tick s))}
-| co_fn : `{let s := (shell (co v σ) ((fn fnv)::κ) t) in
+             red_cesk (shell p κ t) (shell (co (adelay a) σ) κ (tick p σ))}
+| ev_app : `{let p := (ev (app e0 e1) ρ σ) in
+             red_cesk (shell p κ t) (shell (ev e0 ρ σ) ((ar e1 ρ)::κ) (tick p σ))}
+| ev_lam : `{let p := (ev (lam x e) ρ σ) in
+             red_cesk (shell p κ t) (shell (co (closure x e ρ) σ) κ (tick p σ))}
+| co_ar : `{let p := (co v σ) in
+            red_cesk (shell p ((ar e ρ)::κ) t) (shell (ev e ρ σ) ((fn v)::κ) (tick p σ))}
+| co_fn : `{let p := (co v σ) in
             in_force σ (closure x e ρ) fnv ->
-            red_cesk s (shell (ap x e ρ v σ) κ (tick s))}
-| do_ap : `{let s := (shell (ap x e ρ v σ) κ t) in
-            let a := alloc s in
+            red_cesk (shell p ((fn fnv)::κ) t) (shell (ap x e ρ v σ) κ (tick p σ))}
+| do_ap : `{let p := (ap x e ρ v σ) in
+            let a := alloc p σ in
             let ρ' := extend_ρ x a ρ in
             let σ' := σ_join σ a v in
-            red_cesk s (shell (ev e ρ' σ') κ (tick s))}.
+            red_cesk (shell p κ t) (shell (ev e ρ' σ') κ (tick p σ))}.
 
-Section stream.
-  Variable A : Type.
-
-  CoInductive stream : Type :=
-  | Cons : A -> stream -> stream
-  | Nil : stream.
-End stream.
-
-CoInductive Trace {State} (s0 : State) (R : State -> State -> Prop) : stream State -> Prop :=
-  | initial : Trace s0 R (Cons s0 (Nil _))
-  | CESK_step : `{Trace s0 R (Cons ς π) ->
+Inductive Trace {State} (s0 : State) (R : State -> State -> Type) : list State -> Type :=
+  | initial : Trace s0 R (s0 :: nil)
+  | CESK_step : `{Trace s0 R (ς :: π) ->
                   R ς ς' ->
-                  Trace s0 R (Cons ς' (Cons ς π))}.
+                  Trace s0 R (ς' :: (ς :: π))}.
 
 Definition CESK_trace (e : Expr) := Trace (shell (ev e nil nil) nil time0) red_cesk.
 Section NonStandardData.
 Inductive Context :=
-  context : Expr -> Env -> Store -> Context.
+  context : Expr -> Env -> Store -> Time -> Context.
 
 Definition context_eq_dec : dec_type Context.
   decide equality; try solve [apply expr_eq_dec | apply env_eq_dec | apply store_eq_dec].
 Defined.
 
 Inductive Result :=
-  res: val -> Store -> Result.
+  res: val -> Store -> Time -> Result.
 Definition Results := set Result.
 
 Definition result_eq_dec : dec_type Result.
@@ -351,13 +531,24 @@ Definition trunckonts_join (κs κs' : TrunKonts) := set_union trunkont_eq_dec �
 Definition lookup_M := lookup_map context_eq_dec (B := Results).
 Definition lookup_Ξ := lookup_map context_eq_dec (B := TrunKonts).
 
+Definition κs_join := (fun (_ : KTable) κs κ => (set_add trunkont_eq_dec κ κs)).
+Definition κ_singleton := (fun (_ : KTable) κ => singleton trunkont_eq_dec κ).
+Definition res_join := (fun (_ : Memo) rs r => (set_add result_eq_dec r rs)).
+
+Lemma κs_join_extensive (_ : KTable) (b : TrunKonts) (tκ : TrunKont) : InT tκ (set_add trunkont_eq_dec tκ b).
+Proof. apply set_add_intro2T; auto. Qed.
+(*
+Lemma κs_join_extensive' (_ : KTable) (b : TrunKonts) (tκ : TrunKont) := (set_add_intro1 trunkont_eq_dec).
+*)
+Definition κ_singleton_extensive := κs_join_extensive.
+
 Definition Ξ_join (Ξ : KTable) (ctx : Context) (κ : TrunKont) : KTable :=
   list_join context_eq_dec
-            (fun _ κs κ => (set_add trunkont_eq_dec κ κs))
-            (fun _ κ => singleton trunkont_eq_dec κ) Ξ ctx κ Ξ.
+            κs_join
+            κ_singleton Ξ ctx κ Ξ.
 Definition M_join (M : Memo) (ctx : Context) (r : Result) : Memo :=
   list_join context_eq_dec
-            (fun _ rs r => (set_add result_eq_dec r rs))
+            res_join
             (fun _ r => singleton result_eq_dec r) M ctx r M.
 
 Fixpoint map_join {A B} (join1 : list (A * B) -> A -> B -> list (A * B)) (l l' : list (A * B)) :=
@@ -374,10 +565,10 @@ Definition Ms_join := map_join (fun M ctx rs => list_join context_eq_dec
                                                           (fun _ rs => rs)
                                                           M ctx rs M).
 
-Definition in_ctxs (Ξ : KTable) (ctx : Context) (κ : TrunKont) : Prop :=
+Definition in_ctxs (Ξ : KTable) (ctx : Context) (κ : TrunKont) : Type :=
   in_list_list Ξ ctx κ.
 
-Definition in_memos (M : Memo) (ctx : Context) (r : Result) : Prop :=
+Definition in_memos (M : Memo) (ctx : Context) (r : Result) : Type :=
   in_list_list M ctx r.
 
 Inductive WShell (P : Type) :=
@@ -400,133 +591,167 @@ Variable allocmk : CESKMΞ -> Addr.
 Variable tickmk : CESKMΞ -> Time.
 Variable time0mk : Time.
 
-Inductive red_ceskmk : CESKMΞ -> CESKMΞ -> Prop :=
-  evmk_var : `{let s := widemk (wshell (ev (var x) ρ σ) κ t) M Ξ in
+Inductive red_ceskmk : CESKMΞ -> CESKMΞ -> Type :=
+  evmk_var : `{let s := widemk (wshell (ev (var x) ρ σ) tκ t) M Ξ in
              MapsTo ρ x a ->
-             red_ceskmk s (widemk (wshell (co (adelay a) σ) κ (tickmk s))  M Ξ)}
-| evmk_app : `{let s := widemk (wshell (ev (app e0 e1) ρ σ) κ t) M Ξ in
-             red_ceskmk s (widemk (wshell (ev e0 ρ σ) (kpush (ar e1 ρ) κ) (tickmk s)) M Ξ)}
-| evmk_lam : `{let s := widemk (wshell (ev (lam x e) ρ σ) κ t) M Ξ in
-             red_ceskmk s (widemk (wshell (co (closure x e ρ) σ) κ (tickmk s)) M Ξ)}
-| comk_ar : `{let s := widemk (wshell (co v σ) (kpush (ar e ρ) κ) t) M Ξ in
-            red_ceskmk s (widemk (wshell (ev e ρ σ) (kpush (fn v) κ) (tickmk s)) M Ξ)}
-| comk_fn : `{let s := widemk (wshell (co v σ) (kpush (fn fnv) κ) t) M Ξ in
+             red_ceskmk s (widemk (wshell (co (adelay a) σ) tκ (tickmk s))  M Ξ)}
+| evmk_app : `{let s := widemk (wshell (ev (app e0 e1) ρ σ) tκ t) M Ξ in
+             red_ceskmk s (widemk (wshell (ev e0 ρ σ) (kpush (ar e1 ρ) tκ) (tickmk s)) M Ξ)}
+| evmk_lam : `{let s := widemk (wshell (ev (lam x e) ρ σ) tκ t) M Ξ in
+             red_ceskmk s (widemk (wshell (co (closure x e ρ) σ) tκ (tickmk s)) M Ξ)}
+| comk_ar : `{let s := widemk (wshell (co v σ) (kpush (ar e ρ) tκ) t) M Ξ in
+            red_ceskmk s (widemk (wshell (ev e ρ σ) (kpush (fn v) tκ) (tickmk s)) M Ξ)}
+| comk_fn : `{let s := widemk (wshell (co v σ) (kpush (fn fnv) tκ) t) M Ξ in
               in_force σ (closure x e ρ) fnv ->
-              red_ceskmk s (widemk (wshell (ap x e ρ v σ) κ (tickmk s)) M Ξ)}
-| do_apmk : `{let s := widemk (wshell (ap x e ρ v σ) κ t) M Ξ in
+              red_ceskmk s (widemk (wshell (ap x e ρ v σ) tκ (tickmk s)) M Ξ)}
+| do_apmk : `{let s := widemk (wshell (ap x e ρ v σ) tκ t) M Ξ in
               let a := allocmk s in
               let ρ' := extend_ρ x a ρ in
               let σ' := σ_join σ a v in
-              let ctx := (context e ρ' σ') in
-              let Ξ' := Ξ_join Ξ ctx κ in
+              let t' := (tickmk s) in
+              let ctx := (context e ρ' σ' t') in
+              let Ξ' := Ξ_join Ξ ctx tκ in
               Unmapped M ctx ->
-              red_ceskmk s (widemk (wshell (ev e ρ' σ') (rt ctx) (tickmk s)) M Ξ')}
-| do_memo : `{let s := widemk (wshell (ap x e ρ v σ) κ t) M Ξ in
+              red_ceskmk s (widemk (wshell (ev e ρ' σ') (rt ctx) t') M Ξ')}
+| do_memo : `{let s := widemk (wshell (ap x e ρ v σ) tκ t) M Ξ in
               let a := allocmk s in
               let ρ' := extend_ρ x a ρ in
               let σ' := σ_join σ a v in
-              let ctx := (context e ρ' σ') in
-              let Ξ' := Ξ_join Ξ ctx κ in
-              in_memos M ctx (res vm σm) ->
-              red_ceskmk s (widemk (wshell (co vm σm) κ (tickmk s)) M Ξ')} (* XXX: tick? *)
+              let ctx := (context e ρ' σ' t') in
+              let Ξ' := Ξ_join Ξ ctx tκ in
+              in_memos M ctx (res vm σm tm) ->
+              red_ceskmk s (widemk (wshell (co vm σm) tκ tm) M Ξ')} (* XXX: tick? *)
 | do_rt : `{let s := widemk (wshell (co v σ) (rt ctx) t) M Ξ in
-            let M' := M_join M ctx (res v σ) in
-            in_ctxs Ξ ctx κ ->
-            red_ceskmk s (widemk (wshell (co v σ) κ (tickmk s)) M' Ξ)}.
+            let t' := (tickmk s) in
+            let M' := M_join M ctx (res v σ t') in
+            in_ctxs Ξ ctx tκ ->
+            red_ceskmk s (widemk (wshell (co v σ) tκ t') M' Ξ)}.
 
-Inductive Dom_in_Dom {A B C} : list (A * B) -> list (A * C) -> Prop :=
-  | no_dom : `{Dom_in_Dom nil l}
-  | cons_dom : `{(exists b, In (a,b) l')-> Dom_in_Dom l l' -> Dom_in_Dom ((a,b)::l) l'}.
+Inductive Dom_in_Dom {A B C} : list (A * B) -> list (A * C) -> Type :=
+  | no_dom : forall l, Dom_in_Dom nil l
+  | cons_dom : forall a l l' b',
+                 (existsT b, InT (a,b) l') ->
+                 Dom_in_Dom l l' ->
+                 Dom_in_Dom ((a,b')::l) l'.
 
 Lemma In_join : forall A B C (eq_dec: dec_type A) (l l' : list (A * B))
-                        (f : list (A * B) -> B -> C -> B)  g a a' b b',
-                  (forall a b, In (a,b) l -> In (a,b) l') ->
-                  In (a,b) l ->
-                  exists b'', In (a,b'') (list_join eq_dec f g l' a' b' l).
+                        (f : list (A * B) -> B -> C -> B)  g a a' b b'
+                        (Hcontain : (forall a b, InT (a,b) l -> InT (a,b) l'))
+                        (H : InT (a,b) l),
+                  (existsT b'', InT (a,b'') (list_join eq_dec f g l' a' b' l)).
 Proof.
   intros A B C eq_dec l l' f g a a' b b' Hcontain Hin; induction l as [|(a0,b0) l_ IH];
-  inversion Hin;
-  assert (IHneed : forall a b, In (a,b) l_ -> In (a,b) l') by
+  inversion Hin as [(a1,b1) l1|(a1, b1) l1 ? Hin']; subst;
+  assert (IHneed : forall a b, InT (a,b) l_ -> InT (a,b) l') by
       (intros; apply Hcontain; right; auto);
   pose (rec := IH IHneed);
-  [injection H; intros; subst;
-   unfold list_join;
-   destruct (eq_dec a' a) as [Heq | Hneq];[
-     subst; exists (f l' b b')
-    |exists b]; constructor; auto
-  |unfold list_join;
-    destruct (eq_dec a' a0) as [Heq | Hneq];[
-      exists b; right; auto
-           | destruct rec as [b'' Hb'']; auto; exists b''; right; auto]].
+
+  unfold list_join;
+  destruct (eq_dec a' a0) as [Heq | Hneq];
+  try solve [subst; exists (f l' b0 b'); constructor; auto
+            |exists b; constructor; auto
+            |exists b0; constructor; auto
+            |set (rec2 := rec Hin'); inversion rec2 as [b'' ? Hin_];
+             exists b''; right; auto].
 Qed.
 
-Lemma Dom_join : forall A B C D (eq_dec: dec_type A) (l : list (A * B)) (l' : list (A * D))
-                        (f : list (A * D) -> D -> C -> D)  g a b,
-                   Dom_in_Dom l l' -> Dom_in_Dom l (list_join eq_dec f g l' a b l').
+Lemma Dom_join_right : forall A B C D (eq_dec: dec_type A) (l : list (A * B)) (l' : list (A * D))
+                        (f : list (A * D) -> D -> C -> D)  g a c
+                        (Hdom : Dom_in_Dom l l'), Dom_in_Dom l (list_join eq_dec f g l' a c l').
 Proof.
-  intros A B C D eq_dec l l' f g a b Hdom; induction Hdom;
-  constructor;
-  (induction l';[destruct H as [? bad]; inversion bad |]);
+  intros ? ? ? ? ? ? ? ? ? ? ? Hdom; induction Hdom as [|aa l' ll bb Hex]; [|inversion Hex as [dd ? Hwit]];
+  [constructor
+  |].  
+  induction ll as [|(a_,b_) l'_ IHl'_].
+  inversion Hwit.
+  simpl in *; auto.
+  inversion IHHdom; subst.
+  Admitted.
+(*
+  destruct (eq_dec a a_) as [Heq | Hneq]; [subst|].
+  constructor.
+  apply In_join with (b := dd); auto.
+  simpl in *.
+;[destruct H as [? bad]; inversion bad |]);
   [destruct H as [b' Hb'];
     apply In_join with (b := b')|]; auto.
 Qed.
+*)
 
-Definition TraceTo {State} (R : State -> State -> Prop) (s0 s1 : State) : Prop :=
-  exists pi, Trace s0 R (Cons s1 pi).
+Lemma Dom_join_left : forall A B C D (eq_dec: dec_type A) (l l_ : list (A * B)) (l' : list (A * D))
+                        (f : list (A * B) -> B -> C -> B)  g a b
+                        (Hcontain: (forall ab, InT ab l -> InT ab l_)),
+                   Dom_in_Dom l l' ->
+                   (existsT d, MapsTo l' a d) ->
+                   Dom_in_Dom (list_join eq_dec f g l_ a b l) l'.
+Proof.
+  intros A B C D eq_dec l l_ l' f g a b Hcontain Hdom Hex; inversion Hex as [d ? Hin]; induction Hdom as [|? ? ? ? Hex'].
+  constructor; [exists d; apply MapsTo_In |constructor];auto.
+  simpl; destruct (eq_dec a a0) as [Heq|Hneq]; subst; simpl;
+  [constructor; [exists d; apply MapsTo_In|]; auto
+  |inversion Hex' as [d' ? Hin']; constructor; [exists d'|]; auto].
+  apply IHHdom; try solve [intros; apply Hcontain; right; auto|auto].
+Qed.
+
+
+Definition TraceTo {State} (R : State -> State -> Type) (s0 s1 : State) : Type :=
+  existsT π, Trace s0 R (s1 :: π).
 
 Definition step_all (s : CESKMΞ) : set CESKMΞ :=
   match s with
-    | widemk (wshell (ev (var x) ρ σ) κ t) M Ξ  =>
+    | widemk (wshell (ev (var x) ρ σ) tκ t) M Ξ  =>
       match (lookup_ρ x ρ) with
        | None => empty_set _
-       | Some a => singleton ceskmξ_eq_dec (widemk (wshell (co (adelay a) σ) κ (tickmk s)) M Ξ)
+       | Some a => singleton ceskmξ_eq_dec (widemk (wshell (co (adelay a) σ) tκ (tickmk s)) M Ξ)
       end
-    | widemk (wshell (ev (app e0 e1) ρ σ) κ t) M Ξ =>
-      singleton ceskmξ_eq_dec (widemk (wshell (ev e0 ρ σ) (kpush (ar e1 ρ) κ) (tickmk s)) M Ξ)
-    | widemk (wshell (ev (lam x e) ρ σ) κ t) M Ξ =>
-      singleton ceskmξ_eq_dec (widemk (wshell (co (closure x e ρ) σ) κ (tickmk s)) M Ξ)
-    | widemk (wshell (co v σ) (kpush (ar e ρ) κ) t) M Ξ =>
-              singleton ceskmξ_eq_dec (widemk (wshell (ev e ρ σ) (kpush (fn v) κ) (tickmk s)) M Ξ)
-    | widemk (wshell (co v σ) (kpush (fn fnv) κ) t) M Ξ =>
+    | widemk (wshell (ev (app e0 e1) ρ σ) tκ t) M Ξ =>
+      singleton ceskmξ_eq_dec (widemk (wshell (ev e0 ρ σ) (kpush (ar e1 ρ) tκ) (tickmk s)) M Ξ)
+    | widemk (wshell (ev (lam x e) ρ σ) tκ t) M Ξ =>
+      singleton ceskmξ_eq_dec (widemk (wshell (co (closure x e ρ) σ) tκ (tickmk s)) M Ξ)
+    | widemk (wshell (co v σ) (kpush (ar e ρ) tκ) t) M Ξ =>
+              singleton ceskmξ_eq_dec (widemk (wshell (ev e ρ σ) (kpush (fn v) tκ) (tickmk s)) M Ξ)
+    | widemk (wshell (co v σ) (kpush (fn fnv) tκ) t) M Ξ =>
       (* Append forces *)
       fold_right (fun v acc =>
                     match v with
                         closure x e ρ => set_add ceskmξ_eq_dec
-                                                 (widemk (wshell (ap x e ρ v σ) κ (tickmk s)) M Ξ)
+                                                 (widemk (wshell (ap x e ρ v σ) tκ (tickmk s)) M Ξ)
                                                  acc
                       | _ => acc
                  end)
                  (empty_set _)
                  (force σ fnv)
-    | widemk (wshell (ap x e ρ v σ) κ t) M Ξ =>
+    | widemk (wshell (ap x e ρ v σ) tκ t) M Ξ =>
       let a := allocmk s in
       let ρ' := extend_ρ x a ρ in
       let σ' := σ_join σ a v in
-      let ctx := (context e ρ' σ') in
-      let Ξ' := Ξ_join Ξ ctx κ in
+      let t' := (tickmk s) in
+      let ctx := (context e ρ' σ' t') in
+      let Ξ' := Ξ_join Ξ ctx tκ in
       (* both call and use memo table *)
       match (lookup_M ctx M) with
-            | None => singleton ceskmξ_eq_dec (widemk (wshell (ev e ρ' σ') (rt ctx) (tickmk s)) M Ξ')
+            | None => singleton ceskmξ_eq_dec (widemk (wshell (ev e ρ' σ') (rt ctx) t') M Ξ')
             | Some rs =>
               fold_right (fun r acc =>
                             match r with
-                                res vm σm => set_add ceskmξ_eq_dec
-                                                     (widemk (wshell (co vm σm) κ (tickmk s)) M Ξ')
+                                res vm σm tm => set_add ceskmξ_eq_dec
+                                                     (widemk (wshell (co vm σm) tκ tm) M Ξ')
                                                      acc
                             end)
                          (empty_set _)
                          rs
       end
     | widemk (wshell (co v σ) (rt ctx) t) M Ξ =>
-      let M' := M_join M ctx (res v σ) in
+      let t' := (tickmk s) in
+      let M' := M_join M ctx (res v σ t') in
       match (lookup_Ξ ctx Ξ) with
           | None => (empty_set _)
-          | Some κs =>
-            fold_right (fun κ acc =>
+          | Some tκs =>
+            fold_right (fun tκ acc =>
                           set_add ceskmξ_eq_dec
-                                  (widemk (wshell (co v σ) κ (tickmk s)) M' Ξ)
+                                  (widemk (wshell (co v σ) tκ t') M' Ξ)
                                   acc)
-                       (empty_set _) κs
+                       (empty_set _) tκs
       end
     | widemk (wshell (co v σ) mt t) M Ξ => empty_set _
   end.
@@ -548,19 +773,19 @@ Definition smush_steps (s : WCESKMΞ) (M: Memo) (Ξ: KTable) (S : set WCESKMΞ) 
      end)
     (step_all (widemk s M Ξ)) nil nil nil.
 
-Theorem finite_steps : forall s, exists ss : set CESKMΞ, forall s',
-                         red_ceskmk s s' <-> set_In s' ss.
+Theorem finite_steps : forall s, existsT ss : set CESKMΞ, forall s',
+                          (red_ceskmk s s' -> InT s' ss) *
+                          (InT s' ss -> red_ceskmk s s').
 Proof.
   intro s; exists (step_all s); intro s'; split; [intro Hred|intro Hin].
   inversion_clear Hred; simpl; try solve [left; auto|
 rewrite lookup_mapsto with (eq_dec := name_eq_dec) in H;
 unfold lookup_ρ; rewrite H; constructor; auto].
-inversion H.
 Admitted.
 
 Check smush_steps.
 
-Inductive Wide_CESKMΞ : System -> System -> Prop :=
+Inductive Wide_CESKMΞ : System -> System -> Type :=
   | big_step : forall s M Ξ Seen F ss M' Ξ',
                  (wide_step ss M' Ξ') = (smush_steps s M Ξ Seen) ->
                  Wide_CESKMΞ (**) (system Seen (s::F) M Ξ) (**)
@@ -571,57 +796,100 @@ Inductive Wide_CESKMΞ : System -> System -> Prop :=
 
 Definition WCESKMΞ_trace (e : Expr) := Trace (system ((wshell (ev e nil nil) mt time0)::nil) ((wshell (ev e nil nil) mt time0)::nil) nil nil) Wide_CESKMΞ.
 
-(*
-Inductive StackUnroll_gen gen (Ξ : KTable) : Kont -> TrunKont -> set Context -> Prop :=
-  unroll_mt : forall G, StackUnroll_gen gen Ξ nil mt G
-| unroll_push : forall κ tκ (R : gen Ξ κ tκ (empty_set Context) : Prop) φ G, StackUnroll_gen gen Ξ (φ :: κ) (kpush φ tκ) G
-| unroll_rt : forall ctx G tκ κ (R : gen Ξ κ tκ (set_add context_eq_dec ctx G) : Prop),
-                ~ set_In ctx G -> in_ctxs Ξ ctx tκ ->
-                StackUnroll_gen gen Ξ κ (rt ctx) G.
-
-Check monotone3.
-Check (rel3 Kont (fun _ => TrunKont) (fun _ _ => (set Context))).
-
-
-CoInductive StackUnroll (Ξ : KTable) κ tκ G : Prop :=
-| stackunroll_fold (IN : StackUnroll_gen Ξ StackUnroll κ tκ G).
-
-*)
-
-CoInductive StackUnroll (Ξ : KTable) : Kont -> TrunKont -> list Context -> Prop :=
-  unroll_mt : forall G, StackUnroll Ξ nil mt G
-| unroll_push : forall κ tκ φ G, StackUnroll Ξ κ tκ G -> StackUnroll Ξ (φ :: κ) (kpush φ tκ) G
-| unroll_rt : forall ctx G tκ κ,
-                In ctx G ->
-                StackUnroll Ξ κ tκ (remove_one context_eq_dec ctx G) ->
+Inductive StackUnroll (Ξ : KTable) : Kont -> TrunKont -> Type :=
+  unroll_mt : `{StackUnroll Ξ nil mt}
+| unroll_push : forall κ tκ φ, StackUnroll Ξ κ tκ -> StackUnroll Ξ (φ :: κ) (kpush φ tκ)
+| unroll_rt : forall ctx tκ κ,
+                StackUnroll Ξ κ tκ ->
                 in_ctxs Ξ ctx tκ ->
-                StackUnroll Ξ κ (rt ctx) G.
+                StackUnroll Ξ κ (rt ctx).
+
+Ltac textend_map := apply in_list_join2;solve [
+                             intros; apply set_add_intro1T; auto
+                            | intros; apply set_add_intro2T; auto 
+                            | auto].
 
 Theorem unroll_with_extension : forall
-        (Ξ : KTable) (ctx : Context) (κ : Kont) (tκ tκ' : TrunKont) (G G' : list Context)
-        (hyp : StackUnroll Ξ κ tκ G) (Hsub : Sublist context_eq_dec G G'), StackUnroll (Ξ_join Ξ ctx tκ') κ tκ G'.
+        (Ξ : KTable) (ctx : Context) (κ : Kont) (tκ tκ' : TrunKont)
+        (hyp : StackUnroll Ξ κ tκ), StackUnroll (Ξ_join Ξ ctx tκ') κ tκ.
 Proof.
-  cofix; intros Ξ ctx κ tκ tκ' G G' hyp Hsub.
-  inversion hyp; subst;
-  [constructor
-  |apply unroll_push,unroll_with_extension with (G := G)
-  | ]; auto.
-  apply unroll_rt with (tκ := tκ0); [
-  (* In ctx0 G' *)
-  apply sublist_subset in Hsub;
-    unfold Subset in Hsub;
-    rewrite Forall_forall in Hsub;
-    apply Hsub; assumption
-  |apply unroll_with_extension with (G := (remove_one context_eq_dec ctx0 G));
-    [|apply sublist_remove];assumption
-  |(* in_ctxs*)
-    apply in_list_join2; solve [
-                             intros; apply set_add_intro1; auto
-                            | intros; apply set_add_intro2; auto 
-                            | auto]].
+  intros Ξ ctx κ tκ tκ' hyp; induction hyp;[
+    constructor
+   |constructor; assumption
+   |apply unroll_rt with (tκ := tκ); [|textend_map]; auto].
 Qed.
 
-Inductive KontTail : Kont -> Kont -> Prop :=
+Ltac inject_push :=
+  match goal with [H: kpush ?φ0 ?tκ0 = kpush ?φ1 ?tκ1 |- _] => injection H; intros;
+                                                               try (subst φ1 tκ1); try subst end.
+
+Inductive Unroll_inv : KTable -> TrunKont -> Type :=
+  unroll_inv : forall Ξ κ tκ,
+                 StackUnroll Ξ κ tκ ->
+                 (forall ctx tκ', in_ctxs Ξ ctx tκ' -> existsT κ', StackUnroll Ξ κ' tκ') ->
+                 Unroll_inv Ξ tκ.
+
+Lemma unrolling_inv : forall p p' tκ tκ' t t' M M' Ξ Ξ'
+                             (Hstep : red_ceskmk (widemk (wshell p tκ t) M Ξ)
+                                                 (widemk (wshell p' tκ' t') M' Ξ'))
+                             (Hinv : Unroll_inv Ξ tκ),
+                             Unroll_inv Ξ' tκ'.
+Proof with auto.
+  intros; inversion Hstep as [? ? ? ? ? (* <- time *) ? ? ? s0 Hmap Hpeq Hs'eq |
+                      ? ? ? ? ? ? ? ? s0 Hpeq |
+                      ? ? ? ? ? ? ? ? s0 Hpeq Hs'eq |
+                      ? ? ? ? ? ? ? ? s0 Hpeq Hs'eq |
+                      ? ? ? ? ? ? ? ? ? ? s0 Hin_force Hpeq Hs'eq |
+                      ? ? ? ? ? ? ? ? ? s0 a ρ' σ' t0 ctx Ξ0 Hunmapped Hpeq Hs'eq |
+                      ? ? ? ? ? ? ? ? ? ? ? ? ? s0 a ρ' σ' ctx Ξ0 Hin_memos Hpeq Hs'eq |
+                      ? ? ? ? ? ? tκ0 s0 t0 M0 Hin_ctxs Hpeq Hs'eq];
+  inversion Hinv as [? κ ? Hunroll HΞ];
+  try solve [destruct s0; subst; apply unroll_inv with (κ := κ); auto
+            |destruct s0; subst; apply unroll_inv with (κ := ((ar e1 ρ)::κ)); [constructor|];auto
+            |destruct s0; subst; inversion Hunroll as [|κκ|]; subst; 
+             solve [discriminate | apply unroll_inv with (κ := ((fn v)::κκ)); [constructor|];auto]
+            |destruct s0; subst; inversion Hunroll as [|κκ|]; subst; 
+             solve [discriminate | apply unroll_inv with (κ := ((fn fnv)::κκ)); [constructor|];auto]].
+  (* fn -> ap *)
+  destruct s0; inversion Hunroll as [|κκ|]; subst;
+  solve [discriminate
+        |inject_push; exists κκ; auto].
+  (* unmemoized ap *)
+  apply unroll_inv with (κ := κ);[
+  apply unroll_rt with (tκ := tκ);
+  [apply unroll_with_extension
+  |apply in_list_join]; try solve [auto | intros; apply set_add_intro2T; auto]
+    |].
+  intros ctx_ tκ_ Hin_.
+  destruct (in_list_join_set_split context_eq_dec trunkont_eq_dec) 
+       with (l := Ξ) (l' := Ξ) (a := ctx) (a' := ctx_) (c := tκ) (c' := tκ_)
+    as [[? ?]|S1]; auto;
+  [exists κ; apply unroll_with_extension; subst tκ1 Ξ2 ctx_ tκ_; auto
+  |assert (HΞneed : in_ctxs Ξ ctx_ tκ_) by (unfold in_ctxs; subst tκ1 Ξ2; auto);
+    set (mer := (HΞ ctx_ tκ_ HΞneed)); inversion mer as [κ' ? Hκ'];
+    exists κ'; apply unroll_with_extension; auto].
+  (* memoized ap *)
+  subst Ξ0 Ξ' Ξ2 tκ1 p p' t' tκ'.
+  apply unroll_inv with (κ := κ);
+    [apply unroll_with_extension
+    |intros ctx_ tκ_ Hin_;
+      destruct (in_list_join_set_split context_eq_dec trunkont_eq_dec) 
+       with (l := Ξ) (l' := Ξ) (a := ctx) (a' := ctx_) (c := tκ) (c' := tκ_)
+       as [[? ?]|S1]; auto;
+    [subst tκ_; exists κ; apply unroll_with_extension
+    |assert (HΞneed : in_ctxs Ξ ctx_ tκ_) by auto;
+     set (mer := HΞ ctx_ tκ_ HΞneed); inversion mer as [κ' ? HH];
+     solve [exists κ'; apply unroll_with_extension; auto
+           |auto]]]; auto.
+  (* return and memoize *)
+  subst p p' tκ tκ' Ξ'.
+  assert (HΞneed : in_ctxs Ξ ctx tκ0) by auto;
+    set (mer := (HΞ ctx tκ0 HΞneed)); inversion mer as [κ' ? HH]; auto.
+  apply unroll_inv with (κ := κ'); auto.
+Qed.  
+
+(* needs to be proof-relevant for an always-correct replacetail *)
+Inductive KontTail : Kont -> Kont -> Type :=
 | same_tail : `{KontTail κ κ}
 | push_tail : `{KontTail κ κ' -> KontTail κ (φ :: κ')}.
 
@@ -634,93 +902,712 @@ Fixpoint kont_tailp (κ κ' : Kont) : bool :=
                         end
   end.
 
-Lemma kont_tailp_correct : forall κ κ', kont_tailp κ κ' = true <-> KontTail κ κ'.
+Lemma kont_tailp_correct1 : forall κ κ',
+                             kont_tailp κ κ' = true -> KontTail κ κ'.
 Proof.
   induction κ'; simpl;
-  [destruct (kont_eq_dec κ nil); split; intro H; subst; try solve [constructor
-                                                                  |inversion H; contradiction]
-  |destruct (kont_eq_dec κ (a :: κ')) as [Heq|Hneq]; split; intro H; subst; try solve [constructor];
-   [rewrite IHκ' in H; constructor
-   |rewrite IHκ'; inversion H; subst; [contradict Hneq|]]; auto].
+  [destruct (kont_eq_dec κ nil); intro H; subst; try solve [constructor
+                                                           |inversion H; contradiction]
+  |destruct (kont_eq_dec κ (a :: κ')) as [Heq|Hneq]; intro H; subst; try solve [constructor];
+   apply IHκ' in H; constructor]; auto.
 Qed.
 
-CoInductive hastail (κ : Kont) : stream CESK -> Prop :=
-  Nil_tail : hastail κ (Nil _)
+Lemma kont_tailp_correct2 : forall κ κ',
+                              KontTail κ κ' -> kont_tailp κ κ' = true.
+Proof.
+  induction κ'; simpl;
+  [destruct (kont_eq_dec κ nil); intro H; subst; try solve [constructor
+                                                                  |inversion H; contradiction]
+  |destruct (kont_eq_dec κ (a :: κ')) as [Heq|Hneq]; intro H; subst; try solve [constructor];
+   apply IHκ'; inversion H; subst; [contradict Hneq|]; auto].
+Qed.
+
+Lemma kont_tail_nil : `{KontTail nil κ}.
+Proof. induction κ as [|φ κ_ IH]; constructor; auto. Qed.
+
+Lemma kont_tail_cons : forall φ κ κ' (H : KontTail (φ::κ) κ'), KontTail κ κ'.
+Proof.
+  induction κ' as [|φ_ κ_ IH]; intros; inversion H; subst.
+  apply push_tail; constructor.
+  apply push_tail,IH; auto.
+Qed.  
+
+Lemma kont_tail_app : forall κ κ' κ'' (H : KontTail (κ ++ κ') κ''), KontTail κ' κ''.
+Proof.
+  induction κ as [|φ κ_ IH]; intros;
+  simpl in H; auto.
+  apply kont_tail_cons in H; apply IH; auto.
+Qed.
+
+Inductive hastail (κ : Kont) : list CESK -> Type :=
+  Nil_tail : hastail κ nil
 | Cons_tail : forall π p κ' t, hastail κ π -> KontTail κ κ' ->
-                           hastail κ (Cons (shell p κ' t) π).
+                           hastail κ ((shell p κ' t) :: π).
 
-Inductive Inv : CESKMΞ -> Prop :=
-  inv : forall p κ tκ t M Ξ G,
-Dom_in_Dom M Ξ ->
-StackUnroll Ξ κ tκ G ->
-(forall e ρ σ tκ' κ' G',
-in_ctxs Ξ (context e ρ σ) tκ' ->
-StackUnroll Ξ κ' tκ' G' ->
-(exists t', TraceTo red_cesk
-                    (shell (ev e ρ σ) κ' t')
-                    (shell p κ t))
-/\
-(forall v σ'',
-   in_memos M (context e ρ σ) (res v σ'') ->
-   exists pi t' t'', (Trace (shell (ev e ρ σ) κ' t')
-                        red_cesk
-                        (Cons (shell (co v σ'') κ' t'') pi) /\
-                  hastail κ' pi))) ->
-Inv (widemk (wshell p tκ t) M Ξ).
+(* Tail_replacement κorig κtail κreplacement κresult *)
+Inductive Tail_replacement : Kont -> Kont -> Kont -> Kont -> Type :=
+| tail_replacement : `{Tail_replacement κ κ κ'' κ''}
+| push_replacement : `{Tail_replacement κ κ' κ'' κ''' ->
+                       Tail_replacement (φ::κ) κ' κ'' (φ::κ''')}.
 
-Axiom comparable_ticks : forall p κ tκ t M Ξ G,
-                           StackUnroll Ξ κ tκ G ->
+Lemma good_tailrep : forall κorig κtail κrep,
+                       Tail_replacement (κorig++κtail) κtail κrep (κorig ++ κrep).
+Proof.
+  induction κorig as [|φ κ_ IH];
+  intros;[simpl; constructor
+         |].
+  simpl; constructor; apply IH.
+Qed.
+
+Fixpoint replacetail_kont (κ κ' κ'' : Kont) : option Kont :=
+  match (kont_eq_dec κ κ') with
+  | left _ => Some κ''
+  | right _ => match κ with
+               | nil => None
+               | φ::κ_ => match replacetail_kont κ_ κ' κ'' with
+                            | None => None
+                            | Some κ''_ => Some (φ::κ''_)
+                          end
+               end
+  end.
+
+Inductive Good_Kont : Kont -> Kont -> Kont -> Type :=
+  gkont : forall κ κ' κ'' κ''', replacetail_kont κ κ' κ'' =  Some κ''' -> Good_Kont κ κ' κ''.
+
+Definition replacetail_kont_good : forall κ κ' κ'' (Htail : KontTail κ' κ), Good_Kont κ κ' κ''.
+induction κ as [|φ κ_ IH]; intros;
+[exists κ''; inversion Htail; subst; simpl; reflexivity
+|inversion Htail as [|? ? ? Htail']; subst;
+  [(* tail base case: κ = κ' *) exists κ''; unfold replacetail_kont; split_refl kont_eq_dec (φ :: κ_)
+  |destruct (kont_eq_dec (φ :: κ_) κ') as [Heq | Hneq];
+    [subst; exists κ''; unfold replacetail_kont; split_refl kont_eq_dec (φ :: κ_)
+    |set (mumble := IH κ' κ'' Htail');
+      inversion mumble as [? ? ? κ''' Heq]; subst;
+      exists (φ :: κ'''); unfold replacetail_kont; split_refl2 kont_eq_dec (φ :: κ_) κ'; fold replacetail_kont; rewrite Heq]; auto]].
+Defined.
+
+Definition replacetail_state (s : CESK) (κ' κ'' : Kont) :=
+  match s with
+      shell p κ t => match replacetail_kont κ κ' κ'' with
+                         None => None
+                       | Some κ_ => Some (shell p κ_ t)
+                     end
+  end.
+
+Lemma replacetail_state_good : forall s κ' κ'' (Htail : match s with shell p κ t => KontTail κ' κ end),
+                                 existsT s', replacetail_state s κ' κ'' = Some s'.
+Proof.
+  intros; destruct s as [p κ t]; set (good := replacetail_kont_good κ'' Htail);
+  inversion good as [? ? ? κ''' Hgood]; subst;
+  exists (shell p κ''' t);
+  unfold replacetail_state; rewrite Hgood; auto.
+Qed.
+
+Fixpoint replacetail (π : list CESK) (κ' κ'' : Kont) : list (option CESK) :=
+  match π with
+      nil => nil
+    | ς :: π' => (replacetail_state ς κ' κ'') :: (replacetail π' κ' κ'')
+  end.
+
+Theorem replacetail_good : forall (π : list CESK) (κ' κ'' : Kont) (Htail : hastail κ' π),
+  existsT (π' : list CESK), (replacetail π κ' κ'') = (map (@Some CESK) π').
+Proof.
+  induction π; intros.
+  exists nil; simpl; auto.
+  inversion Htail as [|? p κ_ t Htail' κtail]; subst.
+  destruct (replacetail_state_good (shell p κ_ t) κ' κ'' κtail) as [s' Heq].
+  destruct (IHπ κ' κ'' Htail') as [π' Heq'].
+  exists (s' :: π'); simpl.
+  unfold replacetail_state in Heq; rewrite Heq, Heq'; auto.
+Qed.
+
+Lemma no_circular_cons : forall A a (l : list A), l <> a :: l.
+Proof.
+  intros; intro bad;
+  assert (H : length l = S (length l)) by (rewrite bad at 1; simpl; auto);
+  contradict H; omega.
+Qed.
+
+Lemma no_circular_app : forall A (l l' : list A), length l > 0 -> l' <> l ++ l'.
+Proof.
+  intros; intro bad.
+  assert (H' : length l' = (length l) + (length l')) by (rewrite bad at 1; rewrite app_length; reflexivity).
+  contradict H; omega.
+Qed.
+
+(*
+Require Import Setoid.
+
+
+Lemma no_longer_tail_replacement : forall κ κ' κ'' κmore,
+                                     length κmore > 0 ->
+                                     ~ Tail_replacement κ (κmore ++ κ) κ' κ''.
+Proof.
+  induction κ as [|φ κ_].
+  intros; intro bad; inversion bad; rewrite app_nil_r in H2; contradict H; subst; simpl; omega.
+  intros; intro bad; inversion bad; subst.
+  apply no_circular_app in H2; [contradiction|assumption].
+  assert (~ Tail_replacement κ_ ((κmore ++ [φ]) ++ κ_) κ' κ''').
+  apply IHκ_ with (κmore := κmore ++ [φ]).
+  rewrite app_length; omega.
+  rewrite app_assoc_reverse in H0; simpl in H0; contradiction.
+Qed.
+
+Lemma no_longer_tail_replacement2 : forall κ κ' κmore,
+                                      length κmore > 0 ->
+                                      replacetail_kont κ (κmore ++ κ) κ' = None.
+Proof.
+  induction κ as [|φ κ_ IH].
+  intros; simpl; rewrite app_nil_r; destruct κmore; [contradict H;simpl; omega|reflexivity].
+  intros.
+  unfold replacetail_kont.
+  destruct (kont_eq_dec (φ :: κ_) (κmore ++ φ :: κ_)) as [bad|Hneq].
+  apply no_circular_app in bad; [contradiction|auto].
+  fold replacetail_kont.
+  intros.
+  assert (R : κmore ++ φ :: κ_ = κmore ++ [φ] ++ κ_) by (simpl; reflexivity).
+  rewrite R.
+  rewrite app_assoc with (m := [φ]).
+  rewrite IH; [auto| rewrite app_length; omega].
+Qed.
+
+Lemma replace_is_replacement : forall κ κ' κ'' κ''',
+                       (Tail_replacement κ κ' κ'' κ''' <-> replacetail_kont κ κ' κ'' = Some κ''').
+Proof.
+  induction κ as [|φ κ_ IH];
+  [(* base case *)
+  intros; inversion H; subst; split; intro H'; inversion H'; subst; simpl; constructor; auto
+  |
+  intros; inversion H; subst; split; intro H';
+  [(* inversion case 1, first split *)
+  inversion H' as [| foo bar baz qux boo baa]; subst; unfold replacetail_kont; split_refl kont_eq_dec (φ :: κ_);
+    inversion baa; [match goal with [B : ?k = ?f :: ?k |- _] => apply no_circular_cons in B; contradiction end
+                 |subst;apply no_longer_tail_replacement with (κmore := [φ]) in baa; [contradiction|simpl;omega]]
+  (* second split *)
+  |unfold replacetail_kont in H'; split_refl kont_eq_dec (φ :: κ_);
+  injection H'; intros; subst; constructor; auto
+  (* inversion case 2, first split *)
+  |inversion H'; subst;
+   [unfold replacetail_kont; split_refl kont_eq_dec (φ0 :: κ'0)
+   |rewrite IH in H6;
+   apply kont_tail_cons in H; auto]
+  |]].
+
+  unfold replacetail_kont; fold replacetail_kont; rewrite H6;
+  destruct (kont_eq_dec (φ :: κ_) (φ0 :: κ'0)) as [Heq | Hneq];
+    [inversion H0; subst;
+     [apply no_circular_app with (l := [φ0]) in Heq; [contradiction|simpl;omega]
+     |injection Heq; intros; subst;
+      assert (bad : replacetail_kont (φ1 :: κ') (φ0 :: φ1 :: κ') κ'' = None) by
+          (apply no_longer_tail_replacement2 with (κmore := [φ0]); simpl; auto);
+      rewrite bad in H6; discriminate]
+    |auto].
+
+  unfold replacetail_kont in H'; fold replacetail_kont in H'.
+  destruct (kont_eq_dec (φ :: κ_) (φ0 :: κ'0)) as [Heq | Hneq];
+    [injection H'; injection Heq; intros; subst; constructor
+    |].
+  
+  assert (R : exists κ''_, (replacetail_kont κ_ (φ0 :: κ'0) κ'') = Some κ''_).
+  destruct (replacetail_kont κ_ (φ0 :: κ'0) κ'') as [κ''_|];
+    [injection H';intros;subst; exists κ''_; auto
+    |discriminate].
+  destruct R as [κ''_ repeq].
+  assert (R' : φ :: κ''_ = κ''').
+  destruct (replacetail_kont κ_ (φ0 :: κ'0) κ'') as [κ''__|];
+    [injection H'; injection repeq; intros; subst; auto
+    |discriminate].
+  rewrite <- R'.
+  apply push_replacement.
+  rewrite <- IH in repeq; [| apply kont_tail_cons in H]; auto.
+Qed.
+*)  
+
+Inductive ctx_of : TrunKont -> Context -> Type :=
+  | push_ctx : `{ctx_of tκ ctx -> ctx_of (kpush φ tκ) ctx}
+  | rt_ctx : `{ctx_of (rt ctx) ctx}.
+
+Definition ctx_in_dom (Ξ : KTable) (tκ : TrunKont) :=
+  forall ctx : Context, `{ctx_of tκ ctx -> (existsT κs, InT (ctx,κs) Ξ)}.
+
+Inductive Tailed_Trace : forall (κ : Kont) (p : CES_point) (t : Time) (p' : CES_point) (t' : Time), Type :=
+  tailt : `{Trace (shell p κ t)
+                  red_cesk
+                  ((shell p' κ t') :: π)
+            -> (hastail κ' π) -> Tailed_Trace κ p t p' t'}.
+
+Definition Context_inv :=
+  (fun p tκ M Ξ ctx =>
+     match ctx with
+         context e ρ σ t =>
+         forall tκ',
+             exists κ',
+               StackUnroll Ξ κ' tκ'
+               /\
+               (* seems false now... *)
+               (forall κ,
+                  StackUnroll Ξ κ tκ ->
+                  (exists t', TraceTo red_cesk
+                                      (shell (ev e ρ σ) κ' t')
+                                      (shell p κ t)))
+               /\
+             (forall v σ'' t',
+                in_memos M (context e ρ σ t) (res v σ'' t') ->
+                forall κ_irrelevant, Tailed_Trace κ_irrelevant (ev e ρ σ) t (co v σ'') t')
+  end).
+
+(* prove option versions save with hastail so this goes through *)
+
+Lemma step_push_replace : forall p κ t p' φ t' κ' κ'' κ'''
+                                 (Hstep : red_cesk (shell p κ t) (shell p' (φ :: κ) t'))
+                                 (Hrep : replacetail_kont κ κ' κ'' = Some κ'''),
+                          red_cesk (shell p κ''' t) (shell p' (φ :: κ''') t').
+Proof.
+  intros; inversion Hstep;
+  try solve [match goal with [bad : ?κ = ?φ :: ?κ |- _] => apply no_circular_cons in bad; auto; contradiction end
+            |match goal with [bad : ?κ = ?φ :: ?φ0 :: ?κ |- _] =>
+                             apply no_circular_app with (l := [φ; fn fnv]) in bad; [contradiction|simpl;omega] end].
+  (* app push *)
+  subst; apply ev_app.
+Qed.  
+
+Lemma step_ε_replace : forall p κ t p' t' κ' κ'' κ'''
+                              (Hstep : red_cesk (shell p κ t) (shell p' κ t'))
+                              (Hrep : replacetail_kont κ κ' κ'' = Some κ'''),
+                          red_cesk (shell p κ''' t) (shell p' κ''' t').
+Proof.
+  intros; inversion Hstep;
+  try solve [match goal with [bad : ?κ = ?φ :: ?κ |- _] => apply no_circular_cons in bad; auto; contradiction end
+            |match goal with [bad : ?φ :: ?κ = ?κ |- _] => symmetry in bad; apply no_circular_cons in bad; auto; contradiction end
+            |subst p κ t p' t'; constructor; auto].
+Qed.
+  
+Lemma step_pop_replace : forall p κ t p' φ t' κ' κ'' κ'''
+                                 (Hstep : red_cesk (shell p (φ :: κ) t) (shell p' κ t'))
+                                 (Hrep : replacetail_kont κ κ' κ'' = Some κ'''),
+                          red_cesk (shell p (φ :: κ''') t) (shell p' κ''' t').
+Proof.
+  intros; inversion Hstep;
+  try solve [match goal with [bad : ?φ :: ?κ = ?κ |- _] => symmetry in bad; apply no_circular_cons in bad; auto; contradiction end
+            |match goal with [bad : ?φ :: ?φ0 :: ?κ = ?κ |- _] =>
+                             symmetry in bad; apply no_circular_app with (l := [ar e1 ρ; φ0]) in bad; [contradiction|simpl;omega] end
+            |constructor; auto].
+Qed.
+
+Inductive Stack_Action : Kont -> Kont -> Type :=
+  push_action : forall κ φ, Stack_Action κ (φ :: κ)
+| ε_action : forall κ, Stack_Action κ κ
+| pop_action : forall φ κ, Stack_Action (φ :: κ) κ
+| exchange_action : forall φ φ' κ, Stack_Action (φ :: κ) (φ' :: κ).
+
+Lemma step_push_ε_pop : forall p p' κ κ' t t'
+                               (Hstep : red_cesk (shell p κ t) (shell p' κ' t')),
+                          Stack_Action κ κ'.
+Proof.
+  intros; inversion Hstep;
+  [(* var: ε *)apply ε_action
+  |(* app: push (ar e1 ρ) *)apply push_action
+  |(* lam: ε *)apply ε_action
+  |(* co_ar: exchange *)apply exchange_action
+  |(* fn -> ap: pop (fn v) *)apply pop_action
+  |(* ap : ε *)apply ε_action].
+Qed.
+
+Lemma step_replace : forall p p' κ κ' t t' κtail κrep κres
+                            (Hstep : red_cesk (shell p κ t) (shell p' κ' t'))
+                            (Hrep : replacetail_kont κ κtail κrep = Some κres),
+                       match (step_push_ε_pop Hstep) with
+                           push_action κ φ => red_cesk (shell p κ t) (shell p' (φ :: κ) t')
+                         | ε_action κ => red_cesk (shell p κ t) (shell p' κ t')
+                         | pop_action φ κ => red_cesk (shell p (φ :: κ) t) (shell p' κ t')
+                         | exchange_action φ φ' κ => red_cesk (shell p (φ :: κ) t) (shell p' (φ' :: κ) t)
+                       end.
+                     
+
+Lemma stack_irrelevance : forall p κ t π κ' κ''
+                                 (orig : Trace (shell p κ t) red_cesk π)
+                                 (tail0 : KontTail κ' κ)
+                                 (Htail : hastail κ' π),
+                            exists (s : CESK) (π' : list CESK),
+                              (replacetail_state (shell p κ t) κ' κ'') = Some s /\
+                              (replacetail π κ' κ'') = (map (@Some CESK) π') /\
+                              Trace s red_cesk π'.
+Proof.
+  intros; set (use:=replacetail_kont_good κ'' tail0); inversion use as [? ? ? κ_ H_]; subst.
+  exists (shell p κ_ t);
+  induction orig as [|s0 π0 s1 HT ? Hstep].
+  (* Initial *)
+  exists [(shell p κ_ t)]; repeat split;
+  [unfold replacetail_state; rewrite H_
+  |simpl; rewrite H_
+  |constructor]; auto.
+  (* Step *)
+  inversion Htail as [|? pt κt tt Htail' κtail];
+  set (useκ := replacetail_kont_good κ'' κtail); inversion useκ as [? ? ? κt_ Ht_]; subst;
+  destruct (IHorig Htail') as [π' [Hreps [Hrep HT']]];
+  rewrite Hreps;
+  destruct π' as [|[pr κr tr] π''];
+   [inversion HT'
+   |simpl in Hrep; injection Hrep; intros Hrep0 Hrep1; subst;
+    exists ((shell pt κt_ tt) :: (shell pr κr tr) :: π'');
+    repeat split;
+    [simpl; rewrite Ht_; f_equal|constructor];auto].
+  destruct s0 as [pr' κb tr'].
+  assert (Hκrep : replacetail_kont κb κ' κ'' = Some κr) by
+    (simpl in Hrep1; destruct (replacetail_kont κb κ' κ'');[injection Hrep1; intros; subst; auto|discriminate]).
+  simpl in Hrep1; destruct (replacetail_kont κb κ' κ''); [injection Hrep1; intros; subst; clear Hrep1|discriminate].
+  inversion Hstep;
+    try solve [apply step_push_replace | apply step_pop_replace | constructor; auto].
+
+as [x ρ σ κs tx (* <- time *) a s Hmap Hpeq Hs'eq | (* var *)
+                      e0 e1 ρ σ κs ta s Hpeq | (* app *)
+                      x e ρ σ κs tl s Hpeq Hs'eq | (* lam *)
+                      v σ e ρ κs s Hpeq Hs'eq | (* arg *)
+                      v σ fnv κs tf s Hin_force Hpeq Hs'eq | (* fn -> ap *)
+                      x e ρ v σ κs ts s a ρ' σ' Hpeq Hs'eq].
+  exists ((shell (co (adelay a) σ) κt_ (tick s1)) :: π'); repeat split.
+  Focus 2.
+  
+  try solve [simpl in *; rewrite Ht_, Hrep; auto | auto].
+  simpl in *; rewrite Ht_, <- Hrep; unfold replacetail_state. rewrite Ht_; auto.
+  simpl in Hrep; rewrite <- Hrep.
+  unfold replacetail_state.
+  simpl in *. rewrite Ht_; auto.
+  exists ((shell pt κt_ tt) :: π'); repeat split; auto.
+
+  inversion HT' as [|foo bar baz qux moo boo]; subst.
+  
+  exists (
+  set (last:=replacetail_kont_good κ'' κtail); inversion last as [? ? ? κs_ Hs_];
+  exists ((shell pt κs_ tt) :: π'); repeat split;
+   [simpl in *; rewrite Hs_, Hrep; auto
+   |subst].
+  apply initial.
+  inversion Hstep as [x ρ σ κs tx (* <- time *) a s Hmap Hpeq Hs'eq | (* var *)
+                      e0 e1 ρ σ κs ta s Hpeq | (* app *)
+                      x e ρ σ κs tl s Hpeq Hs'eq | (* lam *)
+                      v σ e ρ κs s Hpeq Hs'eq | (* arg *)
+                      v σ fnv κs tf s Hin_force Hpeq Hs'eq | (* fn -> ap *)
+                      x e ρ v σ κs ts s a ρ' σ' Hpeq Hs'eq];
+
+  (* var *)
+  exists (s1 
+  cofix; intros; inversion orig as [Heq|ς H].
+  subst π.
+  inversion Htail as [|? ? ? ? Htail' κtail']; subst.
+(*  set (repd := replacetail_kont κ κ' κ''). *)
+  set (repd_eq := replacetail_kont_good κ'' κtail').
+  inversion repd_eq as [? ? ? κ''' Heq].
+  assert (seq : replacetail_state (shell p κ t) κ' κ'' tail0 = (shell p κ''' t)).
+  simpl; f_equal; auto.
+  subst.
+  destruct (replacetail_kont_good κ'' tail0).
+  rewrite Heq.
+  apply initial with (s0 := (replacetail_state (shell p κ t) κ' κ'' tail0)).
+
+Inductive Inv : CESKMΞ -> Type :=
+  inv : forall p tκ t M Ξ ctx,
+          Dom_in_Dom M Ξ ->
+          ctx_in_dom Ξ tκ ->
+          ctx_of tκ ctx ->
+          (Context_inv p tκ t M Ξ ctx) ->
+          (forall ctx', (exists κs, InT (ctx',κs) Ξ) -> Context_inv p tκ t M Ξ ctx')
+           ->
+          Inv (widemk (wshell p tκ t) M Ξ).
+
+Axiom comparable_ticks : forall p κ tκ t M Ξ,
+                           StackUnroll Ξ κ tκ ->
                            tick (shell p κ t) = tickmk (widemk (wshell p tκ t) M Ξ).
 
 Lemma inv_invariant : forall s s', Inv s -> red_ceskmk s s' -> Inv s'.
 Proof.
   intros s s' Hinv Hstep.
-  inversion Hinv as [? ? ? ? ? ? G Hdom Htail Φ]; subst.
-  Ltac common Φ kont point κ t invG tightenG pushG :=
-      apply (inv (κ := kont) (G := invG)); try solve [apply unroll_push; auto
-                                                  |constructor; auto
-                                                  |auto];
-      intros e' ρ' σ' tκ' κ' G' Htκ' Hunroll;
-      pose (Φrinst := (Φ e' ρ' σ' tκ' κ' G' Htκ' Hunroll));
-      destruct Φrinst as [Φreach Φmemo];
-      destruct Φreach as [t'_ [π Φreach_path]];
-      split;[
-        (* reach *)
-        exists t'_;
-          exists (Cons (shell point κ t) π);
-          constructor; [assumption|
-                        compute;
-                          rewrite <- (comparable_ticks _ _ _ (κ := κ) (G := tightenG));
-                          solve [constructor; auto
-                                    |auto]]
-              |(* memo *) auto].
-  inversion Hstep as [? ? ? ? ? (* <- time *) ? ? ? s0 Hmap Hpeq Hs'eq |
-                      ? ? ? ? ? ? ? ? ? Hpeq |
-                      ? ? ? ? ? ? ? ? s0 Hpeq Hs'eq |
-                      ? ? ? ? ? ? ? ? s0 Hpeq Hs'eq |
-                      ? ? ? ? ? ? ? ? ? ? s0 Hin_force Hpeq Hs'eq |
-                      ? ? ? ? ? ? ? ? ? s0 a ρ' σ' ctx Ξ' Hunmapped Hpeq Hs'eq |
-                      ? ? ? ? ? ? ? ? ? ? ? s0 a ρ' σ' ctx Ξ' Hin_memos Hpeq Hs'eq |
-                      ? ? ? ? ? ? s0 M' Hin_ctxs Hpeq Hs'eq].
+  inversion Hinv as [? ? ? ? ? [ce cρ cσ] Hdom tκctx ctxdom Hctx Φ]; subst.
+  Ltac doinvert Un κ tκ φ H ctx Hin :=
+    inversion Un as [|κ tκ φ H|ctx tκ κ H Hin];
+    try (set (ctx := (context (var 0) (@nil (Name * Addr)) (@nil (Addr * AbsVal))));
+         set (Hin := 0)).
+  Ltac noinvert Un κ tκ φ H ctx Hin := set (κ := (@nil Frame));
+                                       set (tκ := mt);
+                                       set (φ := (ar (var 0) (@nil (Name * Addr))));
+                                       set (H := 0);
+                                       set (ctx := (context (var 0) (@nil (Name * Addr)) (@nil (Addr * AbsVal))));
+                                       set (Hin := 0).
+  Ltac part1 ctx tκctx := apply (inv _ _ (ctx := ctx)); try solve [apply unroll_push; auto
+                           |repeat constructor; auto
+                           |auto
+                           |apply Dom_join_left; firstorder
+                           |apply Dom_join_right; firstorder
+                           |intros blah blorg; apply tκctx; inversion blorg; subst; auto
+                           |inversion Hctx; subst; try solve [discriminate
+                                                              |constructor; auto
+                                                             |auto]].
+  inversion Hstep as [? ρ σ ? ? (* <- time *) ? ? ? s0 Hmap Hpeq Hs'eq | (* var *)
+                      ? ? ρ σ ? ? ? ? ? Hpeq | (* app *)
+                      ? ? ρ σ ? ? ? ? s0 Hpeq Hs'eq | (* lam *)
+                      ? ? σ ? ? ? ? ? s0 Hpeq Hs'eq | (* arg *)
+                      ? ? σ ? ? ? ? ? ? ? s0 Hin_force Hpeq Hs'eq | (* fn -> ap *)
+                      ? ?  ? ? ? ? ? ? s0 a ρ' σ' ctx' Ξ' Hunmapped Hpeq Hs'eq | (* call unmemo'd *)
+                      ? ? ? ? ? ? ? ? ? ? ? s0 a ρ' σ' ctx' Ξ' Hin_memos Hpeq Hs'eq | (* call memo' *)
+                      ? ? ? ? ? ? tκ' s0 M' Hin_ctxs Hpeq Hs'eq]. (* return *)
+  Ltac solve_inner point t reach :=
+    let tκ' := fresh "tκ'" in
+    let cκ := fresh "cκ" in
+    let cunroll := fresh "cunroll" in
+    let creach := fresh "creach" in
+    let cmemo := fresh "cmemo" in
+    let t'_ := fresh "t'_" in
+    let π := fresh "π" in
+    let chκ := fresh "chκ" in
+    let cH := fresh "cH" in
+    split; [assumption
+           |split;[intros chκ cH; destruct (reach chκ) as [t'_ [π ?]];
+                   try solve [auto | constructor; auto];
+                   exists t'_;
+                   exists (Cons (shell point chκ t) π);
+                   constructor; [assumption
+                                |compute; rewrite <- comparable_ticks with (κ := chκ);
+                                 solve [repeat constructor; auto | auto]]
+                  |]];
+    repeat constructor; auto.
   (* Var lookup *)
-  subst; common Φ κ (ev (var x) ρ σ) κ t G G G.
+  subst; part1 (context ce cρ cσ) tκctx. 
+  intro tκ'; destruct (Hctx tκ') as [cκ [cunroll [creach cmemo]]];
+  exists cκ; solve_inner (ev (var x) ρ σ) t creach.
+  intros [cce ccρ ccσ] ccH; pose (Φinst := Φ (context cce ccρ ccσ) ccH); simpl in Φinst.
+  intro tκ'; destruct (Φinst tκ') as [κ' [un' [reach' memo']]];
+  exists κ'; solve_inner (ev (var x) ρ σ) t reach'.
   (* function eval *)
-  subst; common Φ ((ar e1 ρ)::κ) (ev (app e0 e1) ρ σ) κ t G G G.
+  subst; part1 (context ce cρ cσ) tκctx.
+  intro tκ'; destruct (Hctx (kpush (ar e1 ρ) tκ')) as [cκ [cunroll [creach cmemo]]].
+  exists cκ_;
+    split; [assumption
+           |split;[intros chκ cH
+                                                            |]].
+  destruct (creach ((ar e1 ρ)::cκ_)) as [t'_ [π ?]]
+    inversion cH; subst; auto.
+                   try solve [auto | constructor; auto];
+
+
+ solve_inner (ev (app e0 e1) ρ σ) t creach.
+  
+  destruct ctx
+  inversion Hctx; subst; try solve [discriminate
+                                                              |constructor; auto
+                                                             |auto].
+ part2 Φ mumble t idκ; repeat split; auto.
+    let κ_ := fresh "κ_" in
+    let Hunroll_ := fresh "Hunroll_" in    
+    repeat split; auto;
+    intros κ_ Hunroll_;
+    inversion Hunroll_ as [|κ__ ? ? Hu__|]; subst;
+    destruct (mumble κ__) as [t'_ [π Φreach_path]]; auto;
+    exists t'_;
+        exists (Cons (shell (ev (app e0 e1) ρ σ) κ__ t) π);
+        constructor; [assumption|
+                      compute;
+                        rewrite <- (comparable_ticks _ _ _ (κ := κ__));
+                        solve [constructor; auto
+                              |auto]].
   (* lam *)
-  subst; common Φ κ (ev (lam x e) ρ σ) κ t G G G.
-  (* arg eval *)
-  inversion Htail as [|? ? ? ? G'' Hκtail|]; subst;
-  try discriminate;
-  injection H4; intros; subst;
-  common Φ (fn v :: κ1) (co v σ) ((ar e ρ)::κ1) t G G G''.
+  subst; part1; part2 Φ mumble t idκ; repeat split; auto.
+    let κ_ := fresh "κ_" in
+    let Hunroll_ := fresh "Hunroll_" in    
+    repeat split; auto;
+    intros κ_ Hunroll_;
+    destruct (mumble κ_) as [t'_ [π Φreach_path]]; auto;
+    exists t'_;
+        exists (Cons (shell (ev (lam x e) ρ σ) κ_ t) π);
+        constructor; [assumption|
+                      compute;
+                        rewrite <- (comparable_ticks _ _ _ (κ := κ_));
+                        solve [constructor; auto
+                              |auto]].  
+  (* evaluated fn, now arg eval *)
+    subst; part1; part2 Φ mumble t idκ; repeat split; auto;
+    let κ_ := fresh "κ_" in
+    let Hunroll_ := fresh "Hunroll_" in    
+    repeat split; auto;
+    intros κ_ Hunroll_;
+    inversion Hunroll_ as [|κ__|]; subst;
+    destruct (mumble ((ar e ρ)::κ__)) as [t'_ [π Φreach_path]];
+      [constructor|];auto;
+    exists t'_;
+        exists (Cons (shell (co v σ) ((ar e ρ)::κ__) t) π);
+        constructor; [assumption
+                     |compute; rewrite <- (comparable_ticks _ _ _ (κ := ((ar e ρ)::κ__)));
+                      solve [constructor; auto | auto]].
   (* fn -> ap *)
-  inversion Htail as [|? ? ? ? Hκtail|]; subst;
-  try discriminate;
-  injection H4; intros; subst;
-  common Φ κ1 (co v σ) ((fn fnv)::κ1) t G G G.
+    subst; part1; part2 Φ mumble t idκ; repeat split; auto.
+    let κ_ := fresh "κ_" in
+    let Hunroll_ := fresh "Hunroll_" in    
+    repeat split; auto;
+    intros κ_ Hunroll_;
+    destruct (mumble ((fn fnv)::κ_)) as [t'_ [π Φreach_path]];
+    [constructor|]; auto;
+    exists t'_;
+        exists (Cons (shell (co v σ) ((fn fnv)::κ_) t) π);
+        constructor; [assumption|
+                      compute;
+                        rewrite <- (comparable_ticks _ _ _ (κ := ((fn fnv)::κ_)));
+                        solve [constructor; auto
+                              |auto]].
   (* do unmemoized ap *)
-  apply inv with (κ := κ) (G:= G); auto.
-  apply Dom_join; auto.
+    part1.
+    constructor.
+    destruct in_list_join with (eq_dec := context_eq_dec) (combine := κs_join) (base := κ_singleton)
+                                                          (l := Ξ) (l' := Ξ) (a := ctx) (c := tκ)
+                                                          as [κs [? ?]];
+      [intros; apply set_add_intro2T
+       |intros; simpl
+       |
+      |exists κs;apply MapsTo_In]; auto.    
+    let e' := fresh "e'" in
+    let ρ'' := fresh "ρ''" in
+    let σ'' := fresh "σ''" in
+    let tκ' := fresh "tκ'" in
+    let κ' := fresh "κ'" in
+    let Htκ' := fresh "Htκ'" in
+    let Hunroll:= fresh "Hunroll" in
+    intros e' ρ'' σ'' tκ' Htκ'.
+    destruct (in_list_join_set_split context_eq_dec trunkont_eq_dec)
+    with (l := Ξ) (l' := Ξ) (a := ctx) (a' := (context e' ρ'' σ'')) (c := tκ) (c' := tκ')
+                  as [[? ?]|ble];
+      [unfold in_ctxs in Htκ'; auto
+      |(* considered context is the one we extended Ξ with *)
+      subst ctx;
+        match goal with [H : (context ?uu ?vv ?hh) = (context ?ww ?xx ?yy) |- _] =>
+                        injection H; intros aaa bbb ccc; subst ww xx yy end
+      |].
+    inversion Hctx as [HH|? ? HH|? HH].
+    (* mt case *)
+    assert (R : tκ' = mt) by congruence; rewrite R.
+    exists nil; repeat constructor; auto.
+    subst p.
+    pose (mar := Φ e ρ' σ' tκ').
+    
+    
+match goal with [H' : mt = t
+    destruct (Φ e ρ' σ' tκ0) as [stuff boo].
+    injection H3; intros aaa bbb ccc; subst e' ρ'' σ''.
+    
+    [apply in_list_join2
+      |
+      |].
+
+    
+
+    Check in_list_join_split.
+    destruct (in_list_join_split context_eq_dec κs_join κ_singleton) with
+      (l := Ξ)
+      (l' := Ξ)
+      (a := ctx)
+      (a' := (context e' ρ'' σ''))
+      (c := tκ)
+      (c' := tκ') as [S0|[S1|S2]]; auto.
+    destruct (Φ e' ρ'' σ'' tκ' S0) as [κseen [seenunroll [seenreach seenmemo]]].
+    exists κseen; repeat split;
+    [apply unroll_with_extension
+    |intros κreach reachunroll
+    |]; auto.
+
+
+; specialize seenreach with κreach
+ [intros;  | ]; auto.
+.: forall l l' a a' c c'
+                             (Hcontain : (forall ab, InT ab l -> InT ab l')),
+    
+    destruct Φrinst as [κ' [Hunroll [Φreach Φmemo]]].
+    exists (κfn1 κ').
+
+
+ part2 Φ mumble t idκ; repeat split; auto.
+  Focus 3.
+  (* return and memoize *)
+  inversion Htail as [| | ? ? ? Hunroll Hctxin]; subst;
+  [discriminate
+  |discriminate
+  |match goal with [H : rt ?ctx0 = rt ctx |- _] => injection H; intros; subst end].
+  destruct ctx as [e_ ρ_ σ_];
+    destruct (Φ e_ ρ_ σ_ tκ' Hin_ctxs) as [κ' [? [? ?]]].
+
+  apply (inv (κ := κ')); try solve [apply unroll_push; auto
+                                  |constructor; auto
+                                  |auto
+                                  |apply Dom_join_left; firstorder].
+  intros e'' ρ'' σ'' tκ'' Htκ'';
+    pose (Φrinst := (Φ e'' ρ'' σ'' tκ'' Htκ''));
+    destruct Φrinst as [κ'' [Hunroll' [Φreach Φmemo]]];
+    exists κ'';
+    destruct Φreach as [t'_ [π Φreach_path]];
+    repeat split; [auto
+                  |exists t'_|].
+
+ solve [auto |
+      (* reach *)
+      exists t'_;
+        exists (Cons (shell (co v σ) (rt (context e_ ρ_ σ_)) t) π);
+        constructor; [assumption|
+                      compute;
+                        rewrite <- (comparable_ticks _ _ _ (κ := κ));
+                        solve [constructor; auto
+                              |auto]]
+            |(* memo *) auto].
+      part2 Φ point κ t.
+
+  subst; common Φ κ' (co v σ) κ t.
+  
+  constructor.
+  subst; common Φ κ (co v σ) (rt ctx) t.
+
+  apply inv with (κ := κ); auto; subst.
+  (* satisfy hyps of inv first *)
+  apply Dom_join_right; auto.
+  apply unroll_rt with (tκ := tκ); [apply unroll_with_extension; auto
+                                   |apply in_list_join; solve [
+                                                            intros; apply set_add_intro1T; auto
+                                                          | intros; apply set_add_intro2T; auto 
+                                                          | auto]];
+  subst.
+  intros e'' ρ'' σ'' tκ'' κ'' Htκ'' Hunroll'.
+  destruct (in_list_join_split context_eq_dec
+                               κs_join
+                               κ_singleton
+                               κs_join_extensive
+                               Ξ
+                               Ξ
+                               ctx
+                               tκ
+                               (fun a b => b)
+                               (a' := (context e'' ρ'' σ''))
+                               (c' := tκ'')) as [Hctx|[Hctx|Hctx]];
+    auto.
+  (* first case: already there *)
+  pose (Φrinst := (Φ e'' ρ'' σ'' tκ'' κ'' Hctx)).
+    destruct Φrinst as [Φreach Φmemo];
+    destruct Φreach as [t'_ [π Φreach_path]].
+    
+                               Ξ' (* l *)
+                               Ξ' (* l' *)
+                               ctx (* a *)
+                               (context e'' ρ'' σ'') (* a' *)
+                               tκ (* c *)
+                               tκ'' (* c' *).
+  (* unmemoized ap inv needs to split on ctx mapped before or is new *)
+  part2 Φ (ap x e ρ v σ) κ t.
+  inversion Htκ'' as [tκs [Hinp Hinr]].
+  
+
+  pose (Φparinst := (Φ e'' ρ'' σ'' tκ'' κ'' n'')).
+  red in Hinp.
+  pose (Φrinst := ).
+    destruct Φrinst as [Φreach Φmemo];
+    destruct Φreach as [t'_ [π Φreach_path]].
+
+
+  part2 Φ (ap x e ρ v σ) κ t n.
+  (* do memoized ap *)
+  
   assert (Htail' : StackUnroll Ξ' κ tκ (ctx :: G)).
   apply unroll_with_extension with (G := G);[assumption|].
   apply sublist_extension with (l'' := [ ctx ]).
@@ -728,14 +1615,14 @@ Proof.
   apply unroll_rt with (tκ := tκ); try solve [intro bad; inversion bad].
   unfold in_ctxs.
   apply in_list_join; auto;
-  intros; apply set_add_intro2; auto.
+  intros; apply set_add_intro2T; auto.
   pose (Φrinst := (Φ e ρ' σ' (rt ctx) κ' Htκ' Htail));
     destruct Φrinst as [Φreach Φmemo];
     destruct Φreach as [t'_ [π Φreach_path]].
 
-Inductive state_rel : CESK -> System -> Prop :=
+Inductive state_rel : CESK -> System -> Type :=
   point_rel : `{StackUnroll Ξ κ κ' nil ->
-                (set_In (wshell p κ' t) Seen \/ set_In (wshell p κ' t) F) ->
+                (InT (wshell p κ' t) Seen \/ InT (wshell p κ' t) F) ->
                 state_rel (shell p κ t) (system Seen F M Ξ)}.
 
 Theorem simulation : forall e s, CESK_trace e π -> exists s', state_rel s s' /\ WCESKMΞ_trace e π'.
